prove overlay semantics deterministic

theories/overlay/base.v
@@ -1,7 +1,7 @@
 From iris.algebra Require Import base.
 From iris.program_logic Require Import language ectx_language ectxi_language.
 From stdpp Require Import gmap fin_maps list finite.
-From cap_machine Require Export addr_reg machine_base machine_parameters.
+From cap_machine Require Import addr_reg machine_base machine_parameters.
 
 Inductive Cap: Type :=
 | Regular: machine_base.Cap -> Cap (* Regular capabilities *)
@@ -10,10 +10,11 @@ Inductive Cap: Type :=
 
 Instance cap_eq_dec : EqDecision Cap.
 Proof. solve_decision. Defined.
-Instance word_eq_dec : EqDecision Word.
-Proof. solve_decision. Defined.
 
 Definition Word := (Z + Cap)%type.
+
+Instance word_eq_dec : EqDecision Word.
+Proof. solve_decision. Defined.
 
 Notation Reg := (gmap RegName Word).
 Notation Mem := (gmap Addr Word).
@@ -55,6 +56,24 @@ Definition stk (ϕ: ExecConf) :=
 Definition callstack (ϕ: ExecConf) :=
   match ϕ with
   | (_, _, _, cs) => cs
+  end.
+
+Definition update_reg (ϕ: ExecConf) (r: RegName) (w: Word): ExecConf := (<[r:=w]>(reg ϕ), mem ϕ, stk ϕ, callstack ϕ).
+Definition update_mem (φ: ExecConf) (a: Addr) (w: Word): ExecConf := (reg φ, <[a:=w]>(mem φ), stk φ, callstack φ).
+Definition update_stk (φ: ExecConf) (a: Addr) (w: Word): ExecConf := (reg φ, mem φ, <[a:=w]> (stk φ), callstack φ).
+Fixpoint update_callstack (cs: list Stackframe) (d: nat) (a: Addr) (w: Word): option (list Stackframe) :=
+  match cs with
+  | sf::cs => if nat_eq_dec d (length cs) then Some ((fst sf, <[a := w]> (snd sf))::cs)
+             else match update_callstack cs d a w with
+                  | None => None
+                  | Some cs => Some (sf::cs)
+                  end
+  | [] => None
+  end.
+Definition update_stack (φ: ExecConf) (d: nat) (a: Addr) (w: Word): option ExecConf :=
+  match update_callstack (callstack φ) d a w with
+  | None => None
+  | Some cs => Some (reg φ, mem φ, stk φ, cs)
   end.
 
 Lemma ExecConfDestruct:
